sepcomp/semantics_lemmas.v
@@ -8,9 +8,355 @@ Require Import compcert.common.Memory.
 Require Import compcert.common.Events.
 Require Import compcert.common.AST. 
 Require Import compcert.common.Globalenvs.
+Require Import msl.Extensionality. 
 
 Require Import sepcomp.mem_lemmas.
 Require Import sepcomp.semantics.
+
+(********************* Lemmas and definitions related to mem_step ********)
+
+Lemma mem_step_refl m: mem_step m m.
+  apply (mem_step_freelist _ _ nil); trivial.
+Qed. 
+ 
+Lemma mem_step_free: 
+      forall m b lo hi m', Mem.free m b lo hi = Some m' -> mem_step m m'.
+Proof.
+ intros. eapply (mem_step_freelist _ _ ((b,lo,hi)::nil)). 
+ simpl. rewrite H; reflexivity.
+Qed.
+
+Lemma mem_step_store: 
+      forall m ch b a v m', Mem.store ch m b a v = Some m' -> mem_step m m'.
+Proof.
+ intros. eapply mem_step_storebytes. eapply Mem.store_storebytes; eassumption. 
+Qed.
+
+Axiom external_functions_mem_step: forall name sg ge vargs m1 t vres m2,
+  external_functions_sem name sg ge vargs m1 t vres m2 -> mem_step m1 m2.
+
+Axiom inline_assembly_mem_step: forall text sg ge vargs m1 t vres m2,
+  inline_assembly_sem text sg ge vargs m1 t vres m2 -> mem_step m1 m2.
+ 
+Lemma extcall_mem_step ef ge vargs m1 t vres m2:
+  external_call ef ge vargs m1 t vres m2 -> mem_step m1 m2.
+Proof. 
+intros. destruct ef; simpl in *;
+  try (eapply external_functions_mem_step; eassumption);
+  try inv H; try apply mem_step_refl.
+  + inv H0. try apply mem_step_refl.
+      eapply mem_step_store; eassumption.
+  + eapply mem_step_trans.
+      eapply mem_step_alloc; eassumption.
+      eapply mem_step_store; eassumption.
+  + eapply mem_step_free; eassumption. 
+  + eapply mem_step_storebytes; eassumption.
+  + eapply inline_assembly_mem_step; eassumption.
+Qed.
+
+Record memstep_preserve (P:mem -> mem -> Prop) :=
+  { 
+    preserve_trans: forall m1 m2 m3, P m1 m2 -> P m2 m3 -> P m1 m3;
+    preserve_mem: forall m m', mem_step m m' -> P m m'
+  }.
+
+Lemma preserve_refl {P} (HP: memstep_preserve P): forall m, P m m.
+Proof. intros. eapply (preserve_mem _ HP). apply mem_step_refl. Qed.
+
+Lemma preserve_free {P} (HP: memstep_preserve P): 
+      forall m b lo hi m', Mem.free m b lo hi = Some m' -> P m m'.
+Proof.
+ intros. eapply (preserve_mem _ HP). eapply mem_step_free; eauto. Qed.
+
+Theorem preserve_conj {P Q} (HP:memstep_preserve P) (HQ: memstep_preserve Q):
+        memstep_preserve (fun m m' => P m m' /\ Q m m').
+Proof.
+intros. constructor.
++ intros. destruct H; destruct H0. split. eapply HP; eauto. eapply HQ; eauto.
++ intros; split. apply HP; trivial. apply HQ; trivial. 
+Qed.
+
+(*opposite direction appears not to hold*)
+Theorem preserve_impl {A} (P:A -> mem -> mem -> Prop) (Q:A->Prop):
+        (forall a, Q a -> memstep_preserve (P a)) -> memstep_preserve (fun m m' => forall a, Q a -> P a m m').
+Proof.
+intros.
+constructor; intros.
++ eapply H; eauto. 
++ apply H; eauto.
+Qed.
+
+Lemma preserve_exensional {P Q} (HP:memstep_preserve P) (PQ:P=Q): memstep_preserve Q.
+subst; trivial. Qed.
+
+(*opposite direction appears not to hold*)
+Theorem preserve_univ {A} (P:A -> mem -> mem -> Prop):
+        (forall a, memstep_preserve (P a)) -> memstep_preserve (fun m m' => forall a, P a m m').
+Proof. intros.
+eapply preserve_exensional.
+eapply (@preserve_impl A (fun a m m'=> P a m m') (fun a=>True)). 
+intros. apply H. extensionality m. extensionality m'. apply prop_ext. intuition.
+Qed.
+
+Theorem mem_forward_preserve: memstep_preserve mem_forward.
+Proof.
+constructor.
++ apply mem_forward_trans.
++ intros. induction H.
+  eapply storebytes_forward; eassumption. 
+  eapply alloc_forward; eassumption. 
+  eapply freelist_forward; eassumption.
+  eapply mem_forward_trans; eassumption.
+Qed.
+
+Theorem readonly_preserve b: memstep_preserve (fun m m' => mem_forward m m' /\ (Mem.valid_block m b -> readonly m b m')).
+Proof.
+constructor.
++ intros. destruct H; destruct H0. 
+  split; intros. eapply mem_forward_trans; eassumption.
+  eapply readonly_trans; eauto. apply H2. apply H. eassumption.
++ intros; induction H. 
+  - split; intros. eapply storebytes_forward; eassumption.
+    eapply storebytes_readonly; eassumption.
+  - intros. 
+    split; intros. eapply alloc_forward; eassumption.
+    eapply alloc_readonly; eassumption.
+  - intros.
+    split; intros. eapply freelist_forward; eassumption.
+    eapply freelist_readonly; eassumption.
+  - destruct IHmem_step1; destruct IHmem_step2.
+    split. eapply mem_forward_trans; eassumption.
+    intros. eapply readonly_trans. eauto. apply H4. apply H1; eassumption.
+Qed.
+
+Theorem readonly_preserve': 
+   memstep_preserve (fun m m' => mem_forward m m' /\ (forall b, Mem.valid_block m b -> readonly m b m')).
+Proof. 
+eapply preserve_exensional.
+eapply preserve_univ; intros. apply (readonly_preserve a).
+  extensionality m. extensionality m'. apply prop_ext.
+  split; intros. split. eapply H. apply xH. intros. eapply (H b). trivial. 
+  destruct H. split; eauto. 
+Qed.
+
+Lemma storebytes_unch_loc_unwritable b ofs: forall l m m' (L: Mem.storebytes m b ofs l = Some m'),
+      Mem.unchanged_on (loc_not_writable m) m m'.
+Proof.
+intros.
+split; intros.
++ split; intros. 
+  eapply Mem.perm_storebytes_1; eassumption.
+  eapply Mem.perm_storebytes_2; eassumption.
++ rewrite (Mem.storebytes_mem_contents _ _ _ _ _ L).
+  apply Mem.storebytes_range_perm in L.
+  destruct (eq_block b0 b); subst.
+  - destruct (zle ofs ofs0).
+      destruct (zlt ofs0 (ofs + Z.of_nat (length l))).
+        elim H. eapply Mem.perm_max. apply L. omega. 
+      rewrite PMap.gss. apply Mem.setN_other. intros. omega.
+    rewrite PMap.gss. apply Mem.setN_other. intros. omega.
+  - rewrite PMap.gso; trivial.
+Qed.
+
+Lemma unch_on_loc_not_writable_trans m1 m2 m3 
+        (Q : Mem.unchanged_on (loc_not_writable m1) m1 m2)
+        (W : Mem.unchanged_on (loc_not_writable m2) m2 m3)
+        (F:mem_forward m1 m2):
+     Mem.unchanged_on (loc_not_writable m1) m1 m3.
+Proof.
+  destruct Q as [Q1 Q2]. destruct W as [W1 W2].
+  split; intros.
+  - cut (Mem.perm m2 b ofs k p <-> Mem.perm m3 b ofs k p).
+      specialize (Q1 _ _ k p H H0). intuition.
+    apply W1; clear W1. intros N. apply H. apply Q1; trivial. apply F; trivial.
+  -  rewrite W2; clear W2.
+       apply Q2; trivial.
+     intros N; apply H. apply F; trivial. eapply Mem.perm_valid_block; eassumption.
+     apply Q1; trivial. eapply Mem.perm_valid_block; eassumption.
+Qed.
+
+Theorem loc_not_writable_preserve: 
+   memstep_preserve (fun m m' => mem_forward m m' /\ Mem.unchanged_on (loc_not_writable m) m m').
+Proof.
+constructor.
++ intros. destruct H as [F1 Q]; destruct H0 as [F2 W].
+  split; intros. eapply mem_forward_trans; eassumption. clear F2.
+  eapply unch_on_loc_not_writable_trans; eassumption.
++ intros; induction H. 
+  - split; intros. eapply storebytes_forward; eassumption.
+    eapply storebytes_unch_loc_unwritable; eassumption.
+  - split; intros. eapply alloc_forward; eassumption.
+    eapply Mem.alloc_unchanged_on; eassumption. 
+  - split; intros. eapply freelist_forward; eassumption.
+    generalize dependent m.
+    induction l; simpl; intros. inv H. apply Mem.unchanged_on_refl.
+    destruct a. destruct p. 
+    remember (Mem.free m b z0 z) as w. destruct w; inv H. symmetry in Heqw.
+    eapply unch_on_loc_not_writable_trans.
+      eapply Mem.free_unchanged_on. eassumption. 
+        intros i I N. elim N; clear N. 
+        eapply Mem.perm_max. eapply Mem.perm_implies. eapply Mem.free_range_perm; eassumption. constructor.
+      apply IHl; eassumption.
+      eapply free_forward; eassumption.
+  - destruct IHmem_step1; destruct IHmem_step2.
+    split. eapply mem_forward_trans; eassumption.
+    intros. clear H H0 H3. eapply unch_on_loc_not_writable_trans; eassumption. 
+Qed.
+
+Lemma freelist_perm: forall l m m' (L : Mem.free_list m l = Some m') b (B: Mem.valid_block m b)
+      ofs (P': Mem.perm m' b ofs Max Nonempty) k p,
+      Mem.perm m b ofs k p <-> Mem.perm m' b ofs k p.
+Proof. induction l; simpl; intros.
++ inv L; split; trivial.
++ destruct a. destruct p0.
+  remember (Mem.free m b0 z0 z) as w. symmetry in Heqw.
+  destruct w; inv L.
+  specialize (IHl _ _  H0 _ (Mem.valid_block_free_1 _ _ _ _ _ Heqw _ B) _ P' k p).
+  assert (P: Mem.perm m b ofs k p <-> Mem.perm m0 b ofs k p).
+  { clear IHl. destruct (Mem.perm_free_list _ _ _ _ _ _ _ H0 P') as [P ?]; clear H0 P'.
+    destruct (eq_block b0 b); subst.
+    - destruct (zlt ofs z0).
+      * split; intros. apply (Mem.perm_free_1 _ _ _ _ _ Heqw) in H0; eauto.
+        eapply Mem.perm_free_3; eassumption.
+      * destruct (zle z ofs).
+        split; intros. apply (Mem.perm_free_1 _ _ _ _ _ Heqw) in H0; eauto.
+                       eapply Mem.perm_free_3; eassumption.
+        split; intros.
+          eelim (Mem.perm_free_2 _ _ _ _ _ Heqw ofs Max Nonempty); clear Heqw; trivial. omega. 
+        eelim (Mem.perm_free_2 _ _ _ _ _ Heqw ofs Max Nonempty); clear Heqw. omega.
+          eapply Mem.perm_implies. eapply Mem.perm_max. eassumption. constructor.
+    - split; intros.
+      * eapply (Mem.perm_free_1 _ _ _ _ _ Heqw); trivial. intuition.
+      * eapply (Mem.perm_free_3 _ _ _ _ _ Heqw); trivial.
+  }
+  intuition.
+Qed.
+
+Theorem perm_preserve: 
+   memstep_preserve (fun m m' =>  mem_forward m m' /\ forall b, Mem.valid_block m b -> forall ofs, Mem.perm m' b ofs Max Nonempty -> 
+                                  forall k p, Mem.perm m b ofs k p <-> Mem.perm m' b ofs k p).
+Proof. 
+constructor.
++ intros; split. eapply mem_forward_trans. apply H. apply H0.
+  destruct H; destruct H0. intros.
+  assert (M: Mem.perm m1 b ofs k p <-> Mem.perm m2 b ofs k p).
+  - clear H2. apply H1; trivial. apply H0; trivial. apply H; trivial.
+  - clear H1.
+    assert (VB2: Mem.valid_block m2 b). apply H; trivial. 
+    destruct (H2 _ VB2 _ H4 k p); destruct M. split; intros; eauto.
++ intros; induction H. 
+  - split; intros. eapply storebytes_forward; eassumption.
+    split; intros. eapply Mem.perm_storebytes_1; eassumption.
+    eapply Mem.perm_storebytes_2; eassumption.
+  - split; intros. eapply alloc_forward; eassumption.
+    split; intros. eapply Mem.perm_alloc_1; eassumption.
+    eapply Mem.perm_alloc_4; try eassumption.
+    intros N; subst b'. elim (Mem.fresh_block_alloc _ _ _ _ _ H H0).
+  - intros; split. eapply freelist_forward; eassumption. 
+    apply (freelist_perm _ _ _ H).
+  - clear H H0. destruct IHmem_step1; destruct IHmem_step2. 
+    split. eapply mem_forward_trans; eassumption.
+    intros. 
+    assert (M: Mem.perm m b ofs k p <-> Mem.perm m'' b ofs k p).
+    * clear H2. apply H0; trivial. apply H1; trivial. apply H; trivial.
+    * clear H0.
+      assert (VB2: Mem.valid_block m'' b). apply H; trivial.   
+      destruct (H2 _ VB2 _ H4 k p); destruct M. split; intros; eauto.
+Qed.
+
+Lemma memsem_preserves {G C} (s: @MemSem G C) P (HP:memstep_preserve P):
+      forall g c m c' m', corestep s g c m c' m'-> P m m'.
+Proof. intros.
+  apply corestep_mem in H.
+  eapply preserve_mem; eassumption.
+Qed.
+
+Lemma corestep_fwd {C G} (s:@MemSem G C) g c m c' m'
+   (CS:corestep s g c m c' m' ): mem_forward m m'.
+Proof.
+eapply memsem_preserves; try eassumption. apply mem_forward_preserve.
+Qed.
+
+Lemma corestep_rdonly {C G} (s:@MemSem G C) g c m c' m'
+   (CS:corestep s g c m c' m') b (VB:Mem.valid_block m b): readonly m b m'.
+Proof.
+eapply (memsem_preserves s _ readonly_preserve'); eassumption.
+Qed.
+
+(*E-step: Axiomatization of external steps - potentially useful when Memory interface is hardened
+Inductive e_step m m' : Prop :=
+    mem_step_estep: mem_step m m' -> e_step m m'
+  | drop_perm_estep: forall b lo hi p, 
+      Mem.drop_perm m b lo hi p = Some m' -> e_step m m'
+  | change_cur_estep: 
+      (forall b ofs, (Mem.mem_access m) !! b ofs Max = (Mem.mem_access m') !! b ofs Max) ->
+      Mem.unchanged_on (loc_not_writable m) m m' ->
+      (Mem.mem_contents m = Mem.mem_contents m') ->
+      Mem.nextblock m = Mem.nextblock m' -> e_step m m'
+  | estep_trans: forall m'',
+       e_step m m'' -> e_step m'' m' -> e_step m m'.
+
+Lemma e_step_refl m: e_step m m.
+Proof. apply mem_step_estep. apply mem_step_refl. Qed.
+
+Lemma estep_forward m m' (E:e_step m m'): mem_forward m m'.
+Proof.
+induction E.
+apply mem_forward_preserve; eassumption.
++ split; intros.
+    eapply Mem.drop_perm_valid_block_1; eassumption.
+    eapply Mem.perm_drop_4; eassumption.
++ split; intros.
+  unfold Mem.valid_block in *. rewrite H2 in *; assumption.
+  unfold Mem.perm. rewrite H. apply H4.
++ eapply mem_forward_trans; eassumption.
+Qed.
+
+Lemma estep_unch_on_loc_not_writable m m' (E:e_step m m'): Mem.unchanged_on (loc_not_writable m) m m'.
+Proof.
+induction E.
++ apply loc_not_writable_preserve in H. apply H. 
++ unfold Mem.drop_perm in H. 
+  destruct (Mem.range_perm_dec m b lo hi Cur Freeable); inv H; simpl in *.
+  split; simpl; trivial.
+  intros. red in H.
+  unfold Mem.perm; simpl. rewrite PMap.gsspec.
+  destruct (peq b0 b); subst; simpl. 2: intuition.
+  destruct (zle lo ofs); simpl. 2: intuition.
+  destruct (zlt ofs hi); simpl. 2: intuition.
+  elim H. eapply Mem.perm_max. eapply Mem.perm_implies. apply r. omega. constructor.
++ trivial. 
++ eapply unch_on_loc_not_writable_trans; try eassumption. eapply estep_forward; eassumption.
+Qed.
+*)
+(*
+Theorem loadbytes_drop m b lo hi p m' (D:Mem.drop_perm m b lo hi p = Some m'):
+  forall b' ofs, 
+  b' <> b \/ ofs < lo \/ hi <= ofs \/ perm_order p Readable ->
+  Mem.loadbytes m' b' ofs 1 = Mem.loadbytes m b' ofs 1.
+Proof.
+  intros.
+Transparent Mem.loadbytes.
+  unfold Mem.loadbytes.
+  destruct (Mem.range_perm_dec m b' ofs (ofs + 1) Cur Readable). 
+  rewrite pred_dec_true.
+  unfold Mem.drop_perm in D. destruct (Mem.range_perm_dec m b lo hi Cur Freeable); inv D. simpl. auto.
+  red; intros. specialize (Mem.perm_drop_1 _ _ _ _ _ _ D ofs0 Cur); intros.
+    destruct (eq_block b' b); subst.
+      destruct H. eapply Mem.perm_drop_3. eassumption. left; trivial. apply r. trivial.
+      destruct (zlt ofs lo). eapply Mem.perm_drop_3. eassumption. right. omega. apply r. trivial.
+      destruct H. omega. 
+      destruct (zle hi ofs). eapply Mem.perm_drop_3. eassumption. right. omega. apply r. trivial. 
+      destruct H. omega.
+      eapply Mem.perm_implies. apply H1. omega. trivial.
+   eapply Mem.perm_drop_3. eassumption. left; trivial. apply r. omega.
+
+  destruct (Mem.range_perm_dec m' b' ofs (ofs + 1) Cur Readable); trivial.
+  elim n; clear n. red; intros. eapply Mem.perm_drop_4. eassumption. apply r. trivial.
+Qed. 
+*)
+
+(*************************************************************************)
 
 Definition corestep_fun {G C M : Type} (sem : CoreSemantics G C M) :=
   forall (m m' m'' : M) ge c c' c'',
@@ -129,66 +475,69 @@ Section corestepN.
 
 End corestepN.
 
-Section CoopCoreSemLemmas.
-Context {G C: Type}.
-Variable coopsem: CoopCoreSem G C.
+Section memstepN.
+  Context {G C:Type} (M:@MemSem G C) (g:G).
 
-Lemma corestepN_fwd: forall ge c m c' m' n,
-  corestepN coopsem ge n c m c' m' -> 
-  mem_forward m m'.
+Lemma corestepN_mem n: forall c m c' m', corestepN M g n c m c' m' -> mem_step m m'.
+induction n; intros; inv H.
+  apply mem_step_refl.
+  destruct H0 as [m'' [CS CSN]]. eapply mem_step_trans. 
+  eapply corestep_mem; eassumption.
+  eapply IHn; eassumption.
+Qed.
+
+Lemma corestep_plus_mem c m c' m' (H:corestep_plus M g c m c' m'): mem_step m m'.
+destruct H as [n H]. eapply corestepN_mem; eassumption. Qed.
+
+Lemma corestep_star_mem c m c' m' (H:corestep_star M g c m c' m'): mem_step m m'.
+destruct H as [n H]. eapply corestepN_mem; eassumption. Qed.
+
+Lemma memsem_preservesN P (HP: memstep_preserve P)
+      n c m c' m' (H: corestepN M g n c m c' m'): P m m'.
+apply corestepN_mem in H. apply HP; trivial. Qed. 
+
+Lemma memsem_preserves_plus P (HP:memstep_preserve P)
+      c m c' m' (H: corestep_plus M g c m c' m'): P m m'.
+destruct H. apply (memsem_preservesN _ HP) in H; trivial. Qed.
+
+Lemma memsem_preserves_star P (HP:memstep_preserve P)
+      c m c' m' (H: corestep_star M g c m c' m'): P m m'.
+destruct H. apply (memsem_preservesN _ HP) in H; trivial. Qed.
+
+Lemma corestepN_fwd n  c m c' m'
+   (CS:corestepN M g n c m c' m'): mem_forward m m'.
 Proof.
-intros until n; revert c m.
-induction n; simpl; auto.
-inversion 1; apply mem_forward_refl; auto.
-intros c m [c2 [m2 [? ?]]].
-apply mem_forward_trans with (m2 := m2).
-apply corestep_fwd in H; auto.
-eapply IHn; eauto.
+eapply memsem_preservesN; try eassumption. apply mem_forward_preserve.
 Qed.
 
-Lemma corestep_star_fwd: forall g c m c' m'
-  (CS:corestep_star coopsem g c m c' m'), 
-  mem_forward m m'.
-Proof. 
-  intros. destruct CS. 
-  eapply corestepN_fwd. 
-  apply H.
-Qed.
-
-Lemma corestep_plus_fwd: forall g c m c' m'
-  (CS:corestep_plus coopsem g c m c' m'), 
-  mem_forward m m'.
+Lemma corestep_plus_fwd c m c' m'
+   (CS:corestep_plus M g c m c' m'): mem_forward m m'.
 Proof.
-   intros. destruct CS.
-   eapply corestepN_fwd.
-   apply H.
+destruct CS. eapply corestepN_fwd; eassumption.
 Qed.
 
-Lemma corestepN_rdonly: forall ge c m c' m' n,
-  corestepN coopsem ge n c m c' m' -> forall b
-  (VB: Mem.valid_block m b), readonly m b m'.
+Lemma corestep_star_fwd c m c' m'
+   (CS:corestep_star M g c m c' m'): mem_forward m m'.
 Proof.
-intros until n; revert c m.
-induction n; simpl; auto.
-inversion 1; intros. apply readonly_refl.
-intros c m [c2 [m2 [? ?]]].
-intros. apply readonly_trans with (m2 := m2).
-eapply corestep_rdonly; eauto.
-eapply IHn; eauto. eapply corestep_fwd; eauto.
+destruct CS. eapply corestepN_fwd; eassumption.
 Qed.
-
-Lemma corestep_plus_rdonly ge c m c' m'
-  (CS: corestep_plus coopsem ge c m c' m') b
-  (VB: Mem.valid_block m b): readonly m b m'.
+ 
+Lemma corestepN_rdonly n c m c' m'
+    (CS:corestepN M g n c m c' m') b (VB:Mem.valid_block m b): readonly m b m'.
 Proof.
-  destruct CS. eapply corestepN_rdonly; eauto. 
+eapply (memsem_preservesN _ readonly_preserve'); eassumption.
 Qed.
 
-Lemma corestep_star_rdonly ge c m c' m'
-  (CS: corestep_star coopsem ge c m c' m') b
-  (VB: Mem.valid_block m b): readonly m b m'.
+Lemma corestep_plus_rdonly c m c' m'
+   (CS:corestep_plus M g c m c' m') b (VB:Mem.valid_block m b): readonly m b m'.
 Proof.
-  destruct CS. eapply corestepN_rdonly; eauto. 
+destruct CS. eapply corestepN_rdonly; eassumption.
 Qed.
 
-End CoopCoreSemLemmas.
+Lemma corestep_star_rdonly c m c' m'
+   (CS:corestep_star M g c m c' m')b (VB:Mem.valid_block m b): readonly m b m'.
+Proof.
+destruct CS. eapply corestepN_rdonly; eassumption.
+Qed.
+ 
+End memstepN.
